src/ExprUnifySyn.v
@@ -3,7 +3,7 @@ Require Import Expr.
 Require Import ExprUnify.
 Require Import Instantiation.
 
-Module Make (S : Instantiation) <: SyntacticUnifier S.
+Module Make (S : Subst) <: SyntacticUnifier S.
   Section typed.
     Variable types : list type.
 
