src/SimpleBlockInstantiation.v
@@ -1,0 +1,97 @@
+Require Import Instantiation.
+Require Import List.
+Require Import ExtLib.Tactics.Consider.
+Require Import ExtLib.Core.EquivDec.
+Require Import Expr Instantiation.
+Require Import Tactics.
+Require UnfolderTac.
+Require ExprUnify.
+
+Set Implicit Arguments.
+Set Strict Implicit.
+
+Lemma ex_iff : forall T (P P' : T -> Prop),
+  (forall x, P x <-> P' x) ->
+  ((exists x, P x) <-> (exists x, P' x)).
+Proof. split; intuition; destruct H0 as [ x ? ]; exists x; firstorder. Qed.
+
+Theorem existsEach_iff : forall ts a P Q,
+  (forall x, map (@projT1 _ _) x = a -> 
+    (P x <-> Q x)) ->
+  (@existsEach ts a P <-> existsEach a Q).
+Proof.
+  induction a; simpl; intros.
+  { specialize (H nil refl_equal). auto. }
+  { apply ex_iff. intros. rewrite IHa. reflexivity.
+    intros. simpl. eapply H. simpl. f_equal. auto. }
+Qed.
+
+Module Make (SUBST : Subst).
+
+  Section existsSubst.
+    Variable types : list type.
+    Variable funcs : functions types.
+    Variable sub : SUBST.Subst types.
+
+    Fixpoint existsSubst (meta vars : env types) (from : nat) (vals : list tvar) 
+      (ret : env types -> Prop) : Prop :=
+      match vals with
+        | nil => ret meta
+        | t :: ts =>
+          match SUBST.Subst_lookup from sub with
+            | None => 
+              exists x : tvarD types t, 
+                existsSubst (meta ++ existT _ _ x :: nil) vars (S from) ts ret
+            | Some v =>
+              match exprD funcs meta vars v t with
+                | None => 
+                  exists x : tvarD types t, 
+                    existsSubst (meta ++ existT _ _ x :: nil) vars (S from) ts 
+                    (fun g => match exprD funcs g vars v t with
+                                | None => False
+                                | Some y => x = y /\ ret g
+                              end)
+                | Some v => existsSubst (meta ++ existT _ _ v :: nil) vars (S from) ts ret
+              end
+          end
+      end.
+
+  End existsSubst.
+
+
+  Theorem existsSubst_sem : forall ts (funcs : functions ts) sub vals meta_env vars_env from ret,
+    existsSubst funcs sub meta_env vars_env from vals ret <->
+    existsEach vals (fun meta_ext =>
+         SUBST.Subst_equations_to funcs (meta_env ++ meta_ext) vars_env sub from meta_ext
+      /\ ret (meta_env ++ meta_ext)).
+  Proof.
+    induction vals; simpl; intros.
+    { rewrite app_nil_r. intuition. }
+    { consider (SUBST.Subst_lookup from sub); intros.
+      { consider (exprD funcs meta_env vars_env e a); intros.
+        { rewrite IHvals; intuition.
+          { exists t. eapply existsEach_sem in H1. eapply existsEach_sem.
+            destruct H1. exists x. destruct H1. split; try assumption.
+            eapply exprD_weaken with (vars' := nil) (uvars' := existT (tvarD ts) a t :: x) in H0. 
+            rewrite app_nil_r in H0. rewrite H0. simpl in *. 
+            rewrite app_ass in *; simpl in *. intuition. }
+          { destruct H1.
+            apply existsEach_sem in H1. apply existsEach_sem.
+            destruct H1. destruct H1. exists x0. split; auto.
+            consider (exprD funcs (meta_env ++ existT (tvarD ts) a x :: x0) vars_env e a); intros.
+            2: intuition.
+            rewrite app_ass in *; simpl in *.
+            eapply exprD_weaken with (vars' := nil) (uvars' := existT (tvarD ts) a x :: x0) in H0. 
+            rewrite app_nil_r in H0. rewrite H0 in H2. inversion H2; clear H2; subst.
+            intuition subst; intuition. } }
+        { apply ex_iff; intros.
+          rewrite IHvals. 
+          apply existsEach_iff; intros.
+          rewrite app_ass; simpl. 
+          destruct (exprD funcs (meta_env ++ existT (tvarD ts) a x :: x0) vars_env e a); intuition. } }
+      { apply ex_iff; intros.
+        rewrite IHvals. apply existsEach_iff; intros. rewrite app_ass; simpl.
+        intuition. } }
+    Qed.
+
+End Make.
